src/lib/GPU.Base.fsti
@@ -4,6 +4,8 @@ open Pulse.Lib.Pervasives
 open FStar.Tactics.V2
 open FStar.Seq
 open Pulse.Lib.BigStar
+open GPU.SizeT
+open FStar.Mul
 module U32 = FStar.UInt32
 
 (* Token for being in CPU code *)
@@ -12,18 +14,74 @@ val cpu : slprop
 (* Token for being in GPU code *)
 val gpu : slprop
 
-let tid_t = nat
+[@@erasable]
+val tid_t : Type0
 
 (* Token for being a particular thread *)
 val thread_id : tid_t -> slprop
 
+(* Arbitrary *)
+let max_blocks = 1024 * 1024
+(* Hard CUDA limit *)
+let max_threads = 1024
+
+(* How many blocks total in the grid *)
+val gdim_x : tid_t -> (r:U32.t { 0 < r /\ r <= max_blocks })
+(* Which block am I in? *)
+val bidx_x : (etid:tid_t) -> (r:U32.t { r < gdim_x etid })
+
+(* How many threads per block *)
+val bdim_x : tid_t -> (r:U32.t { 0 < r /\ r <= max_threads })
+(* Which thread am I in? *)
+val tidx_x : (etid:tid_t) -> (r:U32.t { r < bdim_x etid })
+
+let thread_index (n: tid_t): GTot (i: nat { i < gdim_x n * bdim_x n }) = (
+  assert ((bidx_x n + 1) * bdim_x n <= gdim_x n * bdim_x n);
+  bidx_x n * bdim_x n + tidx_x n
+)
+let thread_count (n: tid_t): GTot pos = gdim_x n * bdim_x n
+
 ```pulse
 val
-fn block_idx_x () (#n:erased tid_t)
+fn block_idx_x () (#n: tid_t)
   requires thread_id n
   returns  id : U32.t
-  ensures  thread_id n ** pure (n == U32.v id)
-``` 
+  ensures  thread_id n ** pure (id == bidx_x n)
+```
+
+```pulse
+val
+fn block_dim_x () (#n: tid_t)
+  requires thread_id n
+  returns  id : U32.t
+  ensures  thread_id n ** pure (id == bdim_x n)
+```
+
+```pulse
+val
+fn thread_idx_x () (#n: tid_t)
+  requires thread_id n
+  returns  id : U32.t
+  ensures  thread_id n ** pure (id == tidx_x n)
+```
+
+let lemma_mul_lt (a b: nat) (c: nat { a < c }) (d: nat { b <= d /\ d > 0 }): Lemma (a * b < c * d) = ()
+
+```pulse
+fn thread_idx_all () (#n: tid_t)
+  requires thread_id n
+  returns  id : U32.t
+  ensures  thread_id n ** pure (U32.v id == thread_index n /\ U32.v id < max_blocks * max_threads)
+{
+  assert (pure (bidx_x n < 1024 * 1024 /\ tidx_x n < 1024 /\ bdim_x n <= 1024));
+  lemma_mul_lt (U32.v (bidx_x n)) (U32.v (bdim_x n)) (1024 * 1024) 1024;
+  // assert (pure (bidx_x n * tidx_x n < 1024 * 1024 * 1024 /\ bdim_x n <= 1024));
+  let bid = block_idx_x ();
+  let bdim = block_dim_x ();
+  let tid = thread_idx_x ();
+  U32.add (U32.mul bid bdim) tid 
+}
+```
 
 (* f<<<1, 1>>>(...); *)
 ```pulse
@@ -37,19 +95,19 @@ fn launch_kernel_1
   ensures  cpu ** post
 ```
 
-(* f<<<n, 1>>>(...); *)
+(* f<<<nblk, nthr>>>(...); *)
 ```pulse
 val
 fn launch_kernel_n
   (#u1: int)
-  (nthr  : U32.t)
-  (#pre  : (tid:nat{tid < U32.v nthr} -> slprop))
-  (#post : (tid:nat{tid < U32.v nthr} -> slprop))
+  (nblk : U32.t { 0 < nblk /\ nblk <= max_blocks })
+  (nthr : U32.t { 0 < nthr /\ nthr <= max_threads })
+  (#pre #post : (tid:nat{ 0 <= tid /\ tid < (nblk * nthr) } -> slprop))
   (k :
-    (etid:erased nat{etid < U32.v nthr}) ->
-    stt unit (gpu ** thread_id etid ** pre etid)
-             (fun _ -> gpu ** thread_id etid ** post etid)
+    (etid: erased tid_t {gdim_x etid == nblk /\ bdim_x etid == nthr }) ->
+    stt unit (         gpu ** thread_id etid ** pre (thread_index etid))
+             (fun _ -> gpu ** thread_id etid ** post (thread_index etid))
   )
-  requires cpu ** bigstar #u1 0 (U32.v nthr) pre
-  ensures  cpu ** bigstar #u1 0 (U32.v nthr) post
+  requires cpu ** bigstar #u1 0 (nblk * nthr) pre
+  ensures  cpu ** bigstar #u1 0 (nblk * nthr) post
 ```
